src/3d/prelude/EverParse3d.Actions.All.fsti
@@ -10,7 +10,7 @@ noextract
 inline_for_extraction
 val action_field_ptr
       (u:squash (EverParse3d.Actions.BackendFlag.backend_flag == BackendFlagBuffer))
-   : action true_inv eloc_none true ___PUINT8
+   : action true_inv disjointness_trivial eloc_none true ___PUINT8
 
 noextract
 inline_for_extraction
@@ -18,7 +18,7 @@ val action_field_ptr_after
       (u:squash (EverParse3d.Actions.BackendFlag.backend_flag == BackendFlagExtern))
       (sz: FStar.UInt64.t)
       (write_to: bpointer ___PUINT8)
-   : action (ptr_inv write_to) (ptr_loc write_to) false bool // if action returns true, writes some value to write_to. if false, do nothing
+   : action (ptr_inv write_to) disjointness_trivial (ptr_loc write_to) false bool // if action returns true, writes some value to write_to. if false, do nothing
 
 noextract
 inline_for_extraction
@@ -27,10 +27,10 @@ val action_field_ptr_after_with_setter
       (sz: FStar.UInt64.t)
       (#output_loc: eloc)
       (write_to: (___PUINT8 -> Tot (external_action output_loc)))
-   : action true_inv output_loc false bool // if action returns true, writes some value to write_to. if false, do nothing
+   : action true_inv disjointness_trivial output_loc false bool // if action returns true, writes some value to write_to. if false, do nothing
 
 noextract
 inline_for_extraction
 val action_field_pos_32
       (u:squash (EverParse3d.Actions.BackendFlag.backend_flag == BackendFlagBuffer))
-   : action true_inv eloc_none false FStar.UInt32.t
+   : action true_inv disjointness_trivial eloc_none false FStar.UInt32.t
